Sort of working best-first search

src/tactic/auto.lean
@@ -11,9 +11,6 @@ import tactic.core
 -/
 
 /-
-Initial 'MVP': backtracking depth-first search with a database of backwards
-lemmas.
-
 TODO:
 
 - Metavariables need to be reset when we switch between branches of the search
@@ -29,42 +26,158 @@ TODO:
   which is a tiny bit inefficient.
 -/
 
-namespace tactic
-namespace auto
-
-open expr
-open tactic.unsafe
+universes u v w
 
 /-!
 ## Utility stuff
 -/
 
-meta def mvar_context (e : expr) : tactic (list expr) :=
-local_context.to_list <$> type_context.run type_context.get_local_context
+namespace list
+
+def find_and_remove {α} (p : α → Prop) [decidable_pred p] :
+  list α → option (α × list α)
+| [] := none
+| (a :: as) :=
+  if p a
+    then some (a, as)
+    else do
+      (x, as) ← find_and_remove as,
+      pure (x, a :: as)
+
+end list
+
+namespace native.rb_lmap
+
+open native
+
+meta def insert_list {α β} (m : rb_lmap α β) (a : α) (bs : list β) : rb_lmap α β :=
+match rb_map.find m a with
+| none := rb_map.insert m a bs
+| some bs' := rb_map.insert m a (bs ++ bs')
+end
+
+end native.rb_lmap
+
+namespace tactic
+
+meta def duplicate_main_goal_mvar : tactic expr := do
+  tgt ← target,
+  mk_meta_var tgt
+
+/-
+`on_duplicated_goals t` runs the tactic `t` on a copy of the current goals. This
+makes sure that `t` does not assign the goal metavariables.
+-/
+meta def on_duplicated_goals {α} (t : tactic α) : tactic α := do
+  gs ← get_goals,
+  gs' ← gs.mmap mk_meta_var,
+  set_goals gs',
+  finally t (set_goals gs)
+
+end tactic
+
+namespace format
+
+open tactic
+
+meta def unlines : list format → format :=
+intercalate line
+
+meta def nested (n : ℕ) (f : format) : format :=
+if f.is_nil
+  then nil
+  else nest n $ format.line ++ f
+
+meta def of_goal (e : expr) : tactic format :=
+if e.is_mvar
+  then with_local_goals' [e] $ read >>= pp
+  else pp e
+
+end format
+
+namespace tactic
+namespace auto
+
+open expr
+open native
+
+/-!
+## Mock implementation of prio queues
+-/
+
+structure priority_queue (α : Type u) (lt : α → α → bool) :=
+(queue : list α)
+
+namespace priority_queue
+
+variables {α : Type u} {lt : α → α → bool}
+
+def empty : priority_queue α lt :=
+⟨[]⟩
+
+def singleton (a : α) : priority_queue α lt :=
+⟨[a]⟩
+
+def from_list (as : list α) : priority_queue α lt :=
+⟨list.qsort lt as⟩
+
+def is_empty (q : priority_queue α lt) : bool :=
+q.queue.empty
+
+def insert (a : α) (q : priority_queue α lt) : priority_queue α lt :=
+⟨list.qsort lt $ a :: q.queue⟩
+
+def insert_list (as : list α) (q : priority_queue α lt) : priority_queue α lt :=
+⟨list.qsort lt $ as ++ q.queue⟩
+
+def pop_min (q : priority_queue α lt) : option (α × priority_queue α lt) :=
+match q.queue with
+| [] := none
+| (a :: as) := some (a, ⟨as⟩)
+end
+
+def filter (p : α → Prop) [decidable_pred p] (q : priority_queue α lt) :
+  priority_queue α lt :=
+⟨q.queue.filter p⟩
+
+def to_list (q : priority_queue α lt) : list α :=
+q.queue
+
+end priority_queue
 
 /-!
 ## Rules
 -/
 
 meta structure rule :=
+(penalty : ℕ)
 (tac : tactic unit)
+(description : format)
 
 namespace rule
 
+protected meta def to_fmt (r : rule) : format :=
+format.sbracket (_root_.to_fmt r.penalty) ++ format.space ++ r.description
+
+meta instance : has_to_format rule :=
+⟨rule.to_fmt⟩
+
 meta def make_apply (e : expr) : tactic rule :=
-pure { tac := trace! "apply {e}" >> apply e >> pure () }
+pure
+  { tac := apply e >> skip,
+    penalty := 0,
+    description := format! "apply {e}" }
 
-meta def make_const_apply (n : name) : tactic rule :=
-pure { tac := trace! "apply {n}" >> mk_const n >>= apply >> pure () }
+meta def make_const_apply (n : name) : tactic rule := do
+  n ← resolve_constant n,
+  pure
+    { tac := mk_const n >>= apply >> skip,
+      penalty := 0,
+      description := format! "apply {n}" }
 
-meta def apply (r : rule) : tactic unit := do
-  trace "---",
-  trace_state,
-  r ← try_core r.tac,
-  match r with
-  | none := trace "(failed)" >> failed
-  | (some _) := trace_state
-  end
+protected meta def lt (r s : rule) : bool :=
+r.penalty < s.penalty
+
 end rule
 
 /-!
@@ -76,13 +189,19 @@ meta structure rule_set :=
 
 namespace rule_set
 
+protected meta def to_fmt (rs : rule_set) : format :=
+format.unlines $ rs.rules.map rule.to_fmt
+
+meta instance : has_to_format rule_set :=
+⟨rule_set.to_fmt⟩
+
 meta def empty : rule_set :=
 ⟨[]⟩
 
 meta def add (r : rule) (rs : rule_set) : rule_set :=
 ⟨r :: rs.rules⟩
 
-meta def fold {α} (rs : rule_set) (init : α) (f : α → rule → tactic α) : tactic α :=
+meta def mfold {α} (rs : rule_set) (init : α) (f : α → rule → tactic α) : tactic α :=
 rs.rules.mfoldl f init
 
 meta def first {α} (rs : rule_set) (f : rule → tactic α) : tactic α :=
@@ -93,6 +212,9 @@ meta def merge (rs₁ rs₂ : rule_set) : rule_set :=
 
 meta def from_list (rs : list rule) : rule_set :=
 ⟨rs⟩
+
+meta def applicable_rules (rs : rule_set) : tactic (list rule) :=
+pure rs.rules
 
 end rule_set
 
@@ -105,15 +227,19 @@ namespace attr
 meta def declaration_to_rule (decl : name) : tactic rule :=
 rule.make_const_apply decl
 
+meta def declarations_to_rule_set (decls : list name) : tactic rule_set :=
+rule_set.from_list <$> decls.mmap declaration_to_rule
+
 @[user_attribute]
 meta def attr : user_attribute rule_set unit :=
 { name := `auto,
   descr := "Registers a definition as a rule for the auto tactic.",
   cache_cfg := {
-    mk_cache := λ decls, rule_set.from_list <$> decls.mmap declaration_to_rule,
-    dependencies := []
-  },
-}
+    mk_cache := declarations_to_rule_set,
+    dependencies := [] } }
+
+meta def registered_rule_set : tactic rule_set :=
+attr.get_cache
 
 end attr
 
@@ -121,14 +247,457 @@ end attr
 ## Search
 -/
 
-meta def dfs (rs : rule_set) : tactic unit := do
-  attr_rules ← attr.attr.get_cache,
-  let rs := rs.merge attr_rules,
-  trace "===",
-  trace_state,
-  focus1 $ rs.first $ λ rule, do
-    rule.apply,
-    all_goals' dfs
+@[derive decidable_eq]
+meta structure node_id :=
+(to_nat : ℕ)
+
+namespace node_id
+
+protected meta def zero : node_id :=
+⟨0⟩
+
+protected meta def succ : node_id → node_id
+| ⟨n⟩ := ⟨n + 1⟩
+
+protected meta def one : node_id :=
+⟨1⟩
+
+protected meta def lt (n m : node_id) : Prop :=
+n.to_nat < m.to_nat
+
+meta instance : has_lt node_id :=
+⟨node_id.lt⟩
+
+-- Surely there's a less annoying way to write this.
+meta instance : decidable_rel ((<) : node_id → node_id → Prop) :=
+λ n m, (infer_instance : decidable (n.to_nat < m.to_nat))
+
+protected meta def to_fmt (id : node_id) : format :=
+_root_.to_fmt id.to_nat
+
+meta instance : has_to_format node_id :=
+⟨node_id.to_fmt⟩
+
+end node_id
+
+meta structure rule_application :=
+(applied_rule : rule)
+(proof : expr)
+(subgoals : list node_id)
+
+namespace rule_application
+
+protected meta def to_tactic_format (r : rule_application) : tactic format := do
+  proof ← pp r.proof,
+  pure $ r.applied_rule.to_fmt ++ format.nested 2 (format.join
+    [ "proof:",
+      format.nested 2 proof,
+      format.line,
+      "subgoal nodes: " ++ to_fmt r.subgoals ])
+
+meta instance : has_to_tactic_format rule_application :=
+⟨rule_application.to_tactic_format⟩
+
+end rule_application
+
+meta structure node :=
+(goal : expr)
+(num_rules_todo : ℕ)
+(active : list rule_application)
+(proof : option rule_application)
+(unprovable : list rule_application)
+(failed : list rule)
+
+namespace node
+
+protected meta def to_tactic_format (n : node) : tactic format := do
+  goal ← format.of_goal n.goal,
+  active ← format.unlines <$> n.active.mmap pp,
+  unprovable ← format.unlines <$> n.unprovable.mmap pp,
+  proof ←
+    match n.proof with
+    | none := pure ("none" : format)
+    | some p := pp p
+    end,
+  pure $ format.join
+    [ "goal:",
+      format.nested 2 goal,
+      format.line,
+      "number of rules to expand: " ++ to_fmt n.num_rules_todo,
+      format.line,
+      "active rules:",
+      format.nested 2 active,
+      format.line,
+      "proof:",
+      format.nested 2 proof,
+      format.line,
+      "unprovable rules:",
+      format.nested 2 unprovable,
+      format.line,
+      "failed rules:",
+      format.nested 2 $ format.unlines (n.failed.map to_fmt)
+    ]
+
+meta instance : has_to_tactic_format node :=
+⟨node.to_tactic_format⟩
+
+meta def initial (goal : expr) (num_rules_todo : ℕ) : node :=
+{ goal := goal,
+  num_rules_todo := num_rules_todo,
+  failed := [],
+  active := [],
+  unprovable := [],
+  proof := none }
+
+meta def is_proven (n : node) : bool :=
+n.proof.is_some
+
+meta def is_unprovable (n : node) : bool :=
+n.proof.is_none ∧ n.num_rules_todo = 0 ∧ n.active.is_nil
+
+meta def is_unknown (n : node) : bool :=
+n.proof.is_none ∧ (n.num_rules_todo > 0 ∨ ¬ n.active.is_nil)
+
+meta def set_proof (proof : rule_application) (n : node) : node :=
+{ proof := some proof, num_rules_todo := 0, ..n }
+
+end node
+
+/-
+Invariant: All the `node_id`s in `children` and `parents` appear in `nodes`.
+Invariant: The root node has ID `node_id.zero`.
+-/
+meta structure tree :=
+(nodes : rb_map node_id node)
+(parents : rb_map node_id node_id)
+
+namespace tree
+
+meta def singleton (n : node) : tree :=
+{ nodes := rb_map.of_list [(node_id.zero, n)],
+  parents := rb_map.mk _ _ }
+
+meta def contains (id : node_id) (t : tree) : bool :=
+t.nodes.contains id
+
+meta def get (id : node_id) (t : tree) : option node :=
+t.nodes.find id
+
+meta def get' (id : node_id) (err_prefix : format) (t : tree) : tactic node :=
+match t.get id with
+| some n := pure n
+| none := fail $ err_prefix ++ format! "node {id} not found"
+end
+
+meta def get_parent_id (id : node_id) (t : tree) : option node_id :=
+t.parents.find id
+
+meta def get_parent (id : node_id) (t : tree) : option (node_id × node) := do
+  pid ← t.get_parent_id id,
+  p ← t.get pid,
+  pure (pid, p)
+
+meta def get_ancestor_ids : node_id → tree → list node_id := λ id t,
+match t.get_parent_id id with
+| none := []
+| some parent := parent :: get_ancestor_ids parent t
+end
+
+meta def get_ancestors : node_id → tree → list (node_id × node) := λ id t,
+match t.get_parent id with
+| none := []
+| some p@(parent_id, _) := p :: get_ancestors parent_id t
+end
+
+meta def insert (id : node_id) (n : node) (parent : node_id) (t : tree) : tree :=
+{ nodes := t.nodes.insert id n,
+  parents := t.parents.insert id parent }
+
+/- If the node ID doesn't exist yet, it is added. -/
+meta def replace (id : node_id) (n : node) (t : tree) : tree :=
+{ nodes := t.nodes.insert id n, ..t }
+
+meta def rule_application_is_proven (r : rule_application) (t : tree) : bool :=
+r.subgoals.all $ λ id, (node.is_proven <$> t.get id).get_or_else ff
+
+meta def rule_application_is_unprovable (r : rule_application) (t : tree) : bool :=
+r.subgoals.any $ λ id, (node.is_unprovable <$> t.get id).get_or_else tt
+
+meta def propagate_proof_core : list (node_id × node) → tree → tree
+| [] t := t
+| ((id, n) :: ancestors) t :=
+  if n.is_proven
+    then propagate_proof_core ancestors t
+    else
+      match n.active.find_and_remove (λ r, rule_application_is_proven r t) with
+      | some (r, active) :=
+        let t := t.replace id { proof := r, active := active, ..n } in
+        propagate_proof_core ancestors t
+      | none := t
+      end
+
+meta def propagate_proof (id : node_id) (t : tree) : tree :=
+propagate_proof_core (t.get_ancestors id) t
+
+meta def propagate_unprovability_core :
+  rb_set node_id → node_id → tree → tree × rb_set node_id :=
+λ unprovable_nodes id t,
+let recurse_into_parent : rb_set node_id → tree → tree × rb_set node_id :=
+  λ unprovable t,
+  let unprovable := unprovable.insert id in
+  match t.get_parent id with
+  | some (parent, _) :=
+    propagate_unprovability_core unprovable parent t
+  | none := (t, unprovable)
+  end in
+match t.get id with
+| none := (t, unprovable_nodes)
+| some n :=
+  let (unprovable, active) :=
+    n.active.partition $ λ r, rule_application_is_unprovable r t in
+  let n := { active := active, unprovable := n.unprovable ++ unprovable, ..n } in
+  let t := t.replace id n in
+  if n.is_unprovable
+    then
+      let unprovable_nodes := unprovable_nodes.insert id in
+      match t.get_parent id with
+      | some (parent, _) := propagate_unprovability_core unprovable_nodes parent t
+      | none := (t, unprovable_nodes)
+      end
+    else
+      (t, unprovable_nodes)
+end
+
+meta def propagate_unprovability : node_id → tree → tree × rb_set node_id :=
+propagate_unprovability_core (rb_map.mk _ _)
+
+meta def root_node_is_proven (t : tree) : bool :=
+(node.is_proven <$> (t.get node_id.zero)).get_or_else ff
+
+meta def root_node_is_unprovable (t : tree) : bool :=
+(node.is_unprovable <$> (t.get node_id.zero)).get_or_else ff
+
+private meta def link_proofs_core : node_id → tree → tactic unit := λ id t, do
+  (some n) ← pure $ t.get id
+    | fail! "auto/link_proofs: internal error: no node with ID {id}",
+  (some p) ← pure $ n.proof
+    | fail! "auto/link_proofs: internal error: node {id} not proven",
+  p.subgoals.mmap' $ λ subgoal_id, link_proofs_core subgoal_id t,
+  unify n.goal p.proof <|> fail!
+    "auto/link_proofs: internal error: proof of node {id} did not unify with the node goal"
+
+/- Can only be used ONCE after the root node has been proven. -/
+meta def link_proofs : tree → tactic unit :=
+link_proofs_core node_id.zero
+
+/- Only use this after you've called `link_proofs`. -/
+meta def extract_proof (t : tree) : tactic expr := do
+  (some n) ← pure $ t.get node_id.zero
+    | fail "auto/extract_proof: internal error: root node does not exist",
+  instantiate_mvars n.goal
+
+meta def format_node (id : node_id) (n : node) (parent : option node_id) :
+  tactic format := do
+  n ← pp n,
+  pure $ format.join
+    [ "node " ++ to_fmt id,
+      format.nested 2 $ format! "parent: {parent}\n{n}"]
+
+protected meta def to_tactic_format (t : tree) : tactic format :=
+format.unlines <$> t.nodes.to_list.mmap
+  (λ ⟨id, n⟩, format_node id n (t.get_parent_id id))
+
+meta instance : has_to_tactic_format tree :=
+⟨tree.to_tactic_format⟩
+
+end tree
+
+meta structure unexpanded_node :=
+(parent : node_id)
+(rule : rule)
+
+namespace unexpanded_node
+
+protected meta def lt (n m : unexpanded_node) : bool :=
+n.rule.penalty < m.rule.penalty
+
+protected meta def to_fmt (n : unexpanded_node) : format :=
+"for node " ++ n.parent.to_fmt ++ ": " ++ n.rule.to_fmt
+
+meta instance : has_to_format unexpanded_node :=
+⟨unexpanded_node.to_fmt⟩
+
+end unexpanded_node
+
+meta structure state :=
+(search_tree : tree)
+(next_id : node_id)
+(unexpanded_nodes : priority_queue unexpanded_node unexpanded_node.lt)
+
+namespace state
+
+protected meta def to_tactic_format (s : state) : tactic format := do
+  t ← pp s.search_tree,
+  let unexpanded :=
+    format.unlines $ s.unexpanded_nodes.to_list.map unexpanded_node.to_fmt,
+  pure $ format.join
+    [ "search tree:"
+    , format.nested 2 t
+    , format.line
+    , "unexpanded nodes:"
+    , format.nested 2 unexpanded
+    ]
+
+meta instance : has_to_tactic_format state :=
+⟨state.to_tactic_format⟩
+
+end state
+
+meta def initial_state (rs : rule_set) : tactic state := do
+  rules ← rs.applicable_rules,
+  let num_rules_todo := rules.length,
+  let unexpanded_nodes : priority_queue unexpanded_node unexpanded_node.lt :=
+    priority_queue.from_list $ rules.map $ λ r,
+      { parent := node_id.zero, rule := r },
+  goal ← get_goal,
+  pure
+    { search_tree := tree.singleton (node.initial goal num_rules_todo),
+      next_id := node_id.one,
+      unexpanded_nodes := unexpanded_nodes }
+
+meta def run_rule (goal : expr) (r : rule) : tactic (option (expr × list expr)) :=
+with_local_goals' [goal] $ do
+  tgt ← target,
+  goal' ← mk_meta_var tgt,
+  set_goals [goal'],
+  try_core $ do
+    r.tac,
+    subgoals ← get_goals,
+    pure (goal', subgoals)
+
+meta def select_rules (rs : rule_set) (id : node_id) (goal : expr) :
+  tactic (list unexpanded_node) := do
+  rules ← with_local_goals' [goal] $ rs.applicable_rules,
+  pure $ rules.map $ λ r, { parent := id, rule := r }
+
+meta def make_node (rs : rule_set) (s : state) (goal : expr) (parent : node_id) :
+  tactic (node_id × state) := do
+  let id := s.next_id,
+  unexpanded_nodes ← select_rules rs id goal,
+  let node := node.initial goal unexpanded_nodes.length,
+  let s : state :=
+    { next_id := id.succ,
+      unexpanded_nodes := s.unexpanded_nodes.insert_list unexpanded_nodes,
+      search_tree := s.search_tree.insert id node parent },
+  pure (id, s)
+
+meta def make_nodes (rs : rule_set) (s : state) (goals : list expr)
+  (parent : node_id) : tactic (list node_id × state) :=
+goals.mfoldl
+  (λ ⟨ids, s⟩ goal, do
+    (id, s) ← make_node rs s goal parent,
+    pure (id :: ids, s))
+  ([], s)
+
+meta def prune_unexpanded_nodes (parents : rb_set node_id) (s : state) : state :=
+let unexpanded_nodes :=
+  s.unexpanded_nodes.filter (λ n, parents.contains n.parent) in
+{ unexpanded_nodes := unexpanded_nodes, ..s }
+
+meta def expand_node (rs : rule_set) (s : state) (n : unexpanded_node) :
+  tactic state := do
+  let t := s.search_tree,
+  let parent_id := n.parent,
+  let rule := n.rule,
+  (some parent) ← pure $ t.get parent_id
+    | fail "auto/expand_node: internal error: parent of unexpanded node not found",
+  rule_result ← run_rule parent.goal rule,
+  let parent := { num_rules_todo := parent.num_rules_todo - 1, ..parent },
+  s ← match rule_result with
+      | some (prf, []) := do
+          -- Rule succeeded and did not generate subgoals, meaning the parent
+          -- node is proven.
+          -- 1. Record the proof.
+          let rule_app : rule_application :=
+            { applied_rule := rule, proof := prf, subgoals := [] },
+          let parent := parent.set_proof rule_app,
+          -- 2. Potentially mark ancestor nodes as proven.
+          let t :=
+            (t.replace parent_id parent).propagate_proof parent_id,
+          pure { search_tree := t, ..s }
+      | some (prf, subgoals) := do
+          -- Rule succeeded and generated subgoals.
+          -- 1. Make nodes for the subgoals.
+          (subgoal_nodes, s) ← make_nodes rs s subgoals parent_id,
+          -- 2. Add an active rule application with the generated subgoals.
+          let rule_app : rule_application :=
+            { applied_rule := rule, proof := prf, subgoals := subgoal_nodes },
+          let parent := { active := rule_app :: parent.active, ..parent },
+          let t := s.search_tree.replace parent_id parent,
+          pure { search_tree := t, ..s }
+      | none := do
+          -- Rule did not succeed.
+          -- 1. Record rule failure.
+          let parent := { failed := n.rule :: parent.failed, ..parent},
+          let t := s.search_tree.replace parent_id parent,
+          -- 2. Mark nodes which have become unprovable.
+          -- TODO When a node becomes unprovable, its siblings become irrelevant.
+          -- We should check whether a rule belongs to a proven or irrelevant
+          -- node when we apply the rule. That's easier than removing exactly
+          -- the right unexpanded nodes.
+          let (t, _) := t.propagate_unprovability parent_id,
+          pure { search_tree := t, ..s }
+      end,
+  trace "---------------------------------------------------------------------",
+  trace s,
+  pure s
+
+meta def expand (rs : rule_set) (s : state) : tactic (option state) := do
+  trace "=====================================================================",
+  trace s,
+  some (to_expand, unexpanded_nodes) ← pure s.unexpanded_nodes.pop_min
+    | pure none,
+  let s := { unexpanded_nodes := unexpanded_nodes, ..s },
+  (some parent) ← pure $ s.search_tree.get to_expand.parent
+    | fail "auto/expand: internal error: parent of unexpanded node not found",
+  if parent.is_proven
+    then pure (some s)
+    else some <$> expand_node rs s to_expand
+
+meta def finish_if_proven (s : state) : tactic bool := do
+  tt ← pure $ s.search_tree.root_node_is_proven
+    | pure ff,
+  s.search_tree.link_proofs,
+  prf ← s.search_tree.extract_proof,
+  exact prf,
+  pure tt
+
+private meta def search_loop (rs : rule_set) : state → tactic unit := λ s, do
+  ff ← pure $ s.search_tree.root_node_is_unprovable
+    | fail "auto: failed to prove the goal",
+  done ← finish_if_proven s,
+  when ¬ done $ do
+    (some s) ← expand rs s
+      | fail "auto: failed to prove the goal",
+    search_loop s
+
+meta def search (rs : rule_set) : tactic unit :=
+initial_state rs >>= search_loop rs
+
+meta def auto : tactic unit :=
+attr.registered_rule_set >>= search
+
+/-
+TODO
+
+- Purge unexpanded nodes if a sibling rule is proven: it's unnecessary to
+  explore these rules then. (Sibling rules have an OR relationship.)
+- purge subgoals (and their unexpanded nodes) if a sibling goal is unprovable.
+  The parent rule is then unprovable and the siblings don't need to be explored
+  further. (Sibling goals have an AND relationship.)
+- Instead of actually removing these from unexpanded_nodes, we should check
+  whenever we're popping an unexpanded node. Makes the whole thing less horrible.
+-/
 
 end auto
 end tactic
@@ -145,4 +714,4 @@ inductive Even : ℕ → Prop
 
 attribute [auto] Even.zero Even.plus_two
 
-example : Even 6 := by dfs rule_set.empty
+example : Even 6 := by auto
